Lean4Lean/Verify/Environment/Primitive/Gcd.lean
@@ -92,12 +92,12 @@ theorem checkNatGcd.WF {ves : VEnvs} (wf : ves.WF env)
     have hΔ2 := (ctx.withMLC _ (wf := cwf2)).Δwf.toCtx
     have Wc := hcl E γ ih hγ hihT
     have hc := (E.mono <| VEnv.IsDefEqU.app_fun' ctx.Ewf hΔ2
-      (.app_fun' ctx.Ewf hΔ2 hhd hpT haT2) hfT haT).subst Wc
-    have hpT3 := (E.monoT (hhd.of_l ctx.Ewf hΔ2 hpT).hasType.2).subst Wc
+      (.app_fun' ctx.Ewf hΔ2 hhd hpT haT2) hfT haT).subst E.wf.ordered Wc
+    have hpT3 := (E.monoT (hhd.of_l ctx.Ewf hΔ2 hpT).hasType.2).subst E.wf.ordered Wc
     have hfT3 := (E.monoT <| (VEnv.IsDefEqU.app_fun' ctx.Ewf hΔ2 hhd hpT haT2
-      |>.of_l ctx.Ewf hΔ2 hfT).hasType.2).subst Wc
-    have haT3 := (E.monoT haT2).subst Wc
-    have haT3' := (E.monoT haT).subst Wc
+      |>.of_l ctx.Ewf hΔ2 hfT).hasType.2).subst E.wf.ordered Wc
+    have haT3 := (E.monoT haT2).subst E.wf.ordered Wc
+    have haT3' := (E.monoT haT).subst E.wf.ordered Wc
     -- and finally the first argument evaluates: this is what the branch's `Nat.mod` guard buys
     have hmodeq := E.mono (ctx.natBinLit wf.hasPrimitives.natMod hmod a (b+1))
     have hΔ0 : OnCtx [] (E.venv.IsType ctx.lparams.length) := trivial
